\documentclass{article}
\usepackage{amsmath,amssymb}

\title{Deep learning Assignment 4}
\author{Aysha Athar Siddiqui\\
Andrzej Reinke\\
Chang Chun Peng\\
Ramaswamy Venkatachalam\\
Yash Goel
}
\date{December 2020}
\begin{document}
\maketitle
\section{Theory question 1}
Calculating partial derivatives of loss wrt the weights-
The loss function is defined as -
\begin{align}
    L= \sum_{i=1}^{N} (t_i - f(x_i))^{2}
\end{align}
Calculating derivative-\\
\begin{align*}
    \frac{\partial L}{\partial w_j} 
    &= \frac{\partial L}{\partial \sigma} * \frac{\partial \sigma}{\partial O} * \frac{\partial O}{\partial w_j}\\
    \frac{\partial L}{\partial \sigma}
    &=\frac{\partial\sum_{i=1}^{N} (t_i - \sigma(O))^2}{\partial\sigma}
    =\sum_{i=1}^{N}\frac{\partial (t_i - \sigma(O))^2}{\partial \sigma}
    =-2\sum_{i=1}^{N}(t_i-\sigma(O))\\
    \frac{\partial \sigma}{\partial O} 
    &= \frac{\partial (\frac{1}{1+e^{-O}})}{\partial O}
    =-(1+e^{-O})^{-2} * (-e^{-O})
    =\sigma(O)*(1-\sigma (O))\\
    \frac{\partial O}{\partial w_x}
    &=x\\
    \frac{\partial O}{\partial w_y}
    &=y
    \intertext{Hence, Partial derivative wrt $w_x$ and $w_y$ are-}
    \frac{\partial L}{\partial w_x}
    &=-2\sum_{i=1}^{N}(t_i-\sigma(O)) * \sigma(O)*(1-\sigma (O)) * x\\
    \frac{\partial L}{\partial w_y}
    &=-2\sum_{i=1}^{N}(t_i-\sigma(O)) * \sigma(O)*(1-\sigma (O)) * y
\end{align*}
\begin{align*}
    \intertext{\textbf{2nd- SGD without momentum}}
    \intertext{\textbf{First iteration :} }
    O(x,y)
    &=w_x*x+w_y*y=-1*1+1*-1=-2\\
    \sigma(O)
    &=\frac{1}{1+e^{2}}=0.119\\
    \frac{\partial L}{\partial w_x}
    &=-2*(1-0.119)*0.119*(1-0.119)*1=-0.184\\
    \frac{\partial L}{\partial w_y}
    &=-2*(1-0.119)*0.119*(1-0.119)*-1=0.184\\
    w_x
    &=w_x-\alpha*\frac{\partial L}{\partial w_x}=-1-(1)(-0.184)=-0.816\\
    w_y
    &=w_y-\alpha*\frac{\partial L}{\partial w_y}=1-(1)(0.184)=0.816
    \intertext{\textbf{Second iteration}}
    O(x,y)
    &=-0.816*1+0.816*(-1)=-1.632\\
    \sigma(O)
    &=\frac{1}{1+e^{1.632}}=0.163\\
    \frac{\partial L}{\partial w_x}
    &=-2*(1-0.163)*0.163*(1-0.163)*1=-0.228\\
    \frac{\partial L}{\partial w_y}
    &=-2*(1-0.163)*0.163*(1-0.163)*-1=0.228\\
    w_x&=w_x-\alpha*\frac{\partial L}{\partial w_x}=-0.816-(1)(-0.228)=-0.588\\
    w_y&=w_y-\alpha*\frac{\partial L}{\partial w_y}=0.816-(1)(0.228)=0.588
    \intertext{\textbf{Third iteration}}
    O(x,y)&=-0.588*1+0.588*(-1)=-1.176\\
    \sigma(O)
    &=\frac{1}{1+e^{1.176}}=0.235\\
    \frac{\partial L}{\partial w_x}
    &=-2*(1-0.235)*0.235*(1-0.235)*1=-0.275\\
    \frac{\partial L}{\partial w_y}
    &=-2*(1-0.235)*0.235*(1-0.235)*-1=0.275\\
    w_x&=w_x-\alpha*\frac{\partial L}{\partial w_x}=-0.588-(1)(-0.275)=-0.313\\
    w_y&=w_y-\alpha*\frac{\partial L}{\partial w_y}=0.588-(1)(0.275)=0.313
\end{align*}
\textbf{Using Ada-Grad optimization-}
\begin{align*}
    \intertext{\textbf{First iteration :} }
    O(x,y)
    &=w_x*x+w_y*y=-1*1+1*-1=-2\\
    \sigma(O)
    &=\frac{1}{1+e^{2}}=0.119\\
    \frac{\partial L}{\partial w_x}
    &=-2*(1-0.119)*0.119*(1-0.119)*1=-0.184\\
    \frac{\partial L}{\partial w_y}
    &=-2*(1-0.119)*0.119*(1-0.119)*-1=0.184\\
    r_x&=0+(-0.184)*(-0.184)=0.0338\\
    r_y&=0+0.184*0.184=0.0338\\
    \Delta w_x&=-\frac{\varepsilon}{\sqrt{\delta + r}}*g=-\frac{1}{\sqrt{10^{-8}+0.0338}}*-0.184=-\frac{1}{0.183}*-0.184=-5.464*-0.184=1.005 \\
    \Delta w_y&=-\frac{\varepsilon}{\sqrt{\delta + r}}*g=-\frac{1}{\sqrt{10^{-8}+0.0338}}*0.184=-\frac{1}{0.183}*0.184=-5.464*0.184=-1.005\\
    w_x&=-1+1.005=0.005\\
    w_y&=1-1.005=-0.005 
    \intertext{\textbf{Second iteration}}
    O(x,y)
    &=w_x*x+w_y*y=0.005*1+(-0.005)*-1=0.01\\
    \sigma(O)
    &=\frac{1}{1+e^{-0.01}}=0.502\\
    \frac{\partial L}{\partial w_x}
    &=-2*(1-0.502)*0.502*(1-0.502)*1=-0.248\\
    \frac{\partial L}{\partial w_y}
    &=-2*(1-0.502)*0.502*(1-0.502)*-1=0.248\\
    r_x
    &=0.0338+(-0.248)*(-0.248)=0.095\\
    r_y
    &=0.0338+0.248*0.248=0.095
    \Delta w_x
    &=-\frac{\varepsilon}{\sqrt{\delta + r}}*g=-\frac{1}{\sqrt{10^{-8}+0.095}}*-0.248=-\frac{1}{0.308}*-0.248=-3.246*-0.248=0.805\\
    \Delta w_y
    &=-\frac{\varepsilon}{\sqrt{\delta + r}}*g=-\frac{1}{\sqrt{10^{-8}+0.095}}*0.248=-\frac{1}{0.308}*0.248=-3.246*0.248=-0.805\\
    w_x&=0.005+0.805=0.81\\
    w_y&=-0.005-0.805=-0.81\\
    \intertext{\textbf{Third iteration :} }
    O(x,y)
    &=w_x*x+w_y*y=0.81*1+(-0.81)*-1=-1.62\\
    \sigma(O)
    &=\frac{1}{1+e^{-1.62}}=0.835\\
    \frac{\partial L}{\partial w_x}
    &=-2*(1-0.835)*0.835*(1-0.835)*1=-0.045\\
    \frac{\partial L}{\partial w_y}
    &=-2*(1-0.835)*0.835*(1-0.835)*-1=0.045\\
    r_x
    &=0.095+(-0.045)*(-0.045)=0.097\\
    r_y
    &=0.095+0.045*0.045=0.097
    \Delta w_x
    &=-\frac{\varepsilon}{\sqrt{\delta + r}}*g=-\frac{1}{\sqrt{10^{-8}+0.097}}*-0.045=-\frac{1}{0.311}*-0.045=-3.215*-0.045=0.144\\
    \Delta w_y
    &=-\frac{\varepsilon}{\sqrt{\delta + r}}*g=-\frac{1}{\sqrt{10^{-8}+0.097}}*0.045=-\frac{1}{0.311}*0.045=-3.215*0.045=-0.144
    w_x&=0.81+0.144=0.954\\
    w_y&=-0.81-0.144=-0.954
\end{align*}
\textbf{RMSProp - No Momentum with decay rate 0.9 $\rho$}
\begin{align*}
    \intertext{\textbf{First iteration :} }
    O(x,y)
    &=w_x*x+w_y*y=-1*1+1*-1=-2\\
    \sigma(O)
    &=\frac{1}{1+e^{2}}=0.119\\
    \frac{\partial L}{\partial w_x}
    &=-2*(1-0.119)*0.119*(1-0.119)*1=-0.184\\
    \frac{\partial L}{\partial w_y}
    &=-2*(1-0.119)*0.119*(1-0.119)*-1=0.184
    \intertext{Accumulate squared gradient for $w_x$}
    r&=\rho*r+(1-\rho)g*g\\
    r
    &=0+(1-0.9)(-0.184)*(-0.184)=0.00338
    \intertext{Accumulate squared gradient for $w_y$}
    r
    &=0+(1-0.9)0.184*0.184=0.0338\\
    \Delta w_x
    &=-\frac{\varepsilon}{\sqrt{\delta + r}}*g=-\frac{1}{\sqrt{10^{-8}+0.00338}}*-0.184=-\frac{1}{0.058}*-0.184=-17.241*-0.184=3.172 \\
    \Delta w_y
    &=-\frac{\varepsilon}{\sqrt{\delta + r}}*g=-\frac{1}{\sqrt{10^{-8}+0.00338}}*0.184=-\frac{1}{0.058}*0.184=-17.241*0.184=-3.172\\
    w_x
    &=-1+3.172=2.172\\
    w_y
    &=1-3.172=-2.172 
    \intertext{\textbf{Second iteration :} }
    O(x,y)
    &=w_x*x+w_y*y=2.172*1+(-2.172)*-1=4.344\\
    \sigma(O)
    &=\frac{1}{1+e^{-4.344}}=0.987\\
    \frac{\partial L}{\partial w_x}
    &=-2*(1-0.987)*0.987*(1-0.987)*1=-0.00033\\ 
    \frac{\partial L}{\partial w_y}
    &=-2*(1-0.987)*0.987*(1-0.987)*-1=0.00033\\
    r_x
    &=0.9*0.00338+(1-0.9)(-0.00033)*(-0.00033)=0.00304 
    r_y
    &=0.9*0.0338+(1-0.9)(0.00033)*(0.00033)=0.00304\\ 
    \Delta w_x
    &=-\frac{1}{\sqrt{10^{-8}+0.00304}}*-0.248=-\frac{1}{0.055}*-0.00033=-18.181*-0.00033=0.00599 \\
    \Delta w_y
    &=-\frac{1}{\sqrt{10^{-8}+0.00304}}*0.248=-\frac{1}{0.055}*0.00033=-18.181*0.00033=-0.00599\\
    w_x
    &=2.172+0.00599=2.17799\\
    w_y
    &=-2.172-0.00599=-2.17799
    \intertext{\textbf{Third iteration :} }
    O(x,y)
    &=w_x*x+w_y*y=2.17799*1+(-2.17799)*-1=4.355\\
    \sigma(O)
    &=\frac{1}{1+e^{-4.355}}=0.9873\\
    \frac{\partial L}{\partial w_x}
    &=-2*(1-0.9873)*0.9873*(1-0.9873)*1=-0.000318\\ 
    \frac{\partial L}{\partial w_y}
    &=-2*(1-0.9873)*0.9873*(1-0.9873)*-1=0.000318\\
    r_x
    &=0.9*0.00304+(1-0.9)(-0.000318)*(-0.000318)=0.00273\\
    r_y
    &=0.9*0.00304+(1-0.9)(0.000318)*(0.000318)=0.00273\\
    \Delta w_x
    &=-\frac{1}{\sqrt{10^{-8}+0.00273}}*-0.000318=-\frac{1}{0.052}*-0.000318=-19.230*-0.000318=0.0061 \\
    \Delta w_y
    &=-\frac{1}{\sqrt{10^{-8}+0.00273}}*0.000318=-\frac{1}{0.052}*0.000318=-19.230*0.000318=-0.0061\\
    w_x
    &=2.17799+0.0061=2.184\\
    w_y
    &=-2.17799-0.0061=-2.184 
\end{align*}
\textbf{Adam with default decay rate, $\rho1$=0.9 and $\rho2$=0.99}
\begin{align*}
   \intertext{\textbf{For 1st iteration}}
    O(x,y)
    &=w_x*x+w_y*y=-1*1+1*-1=-2\\
    \sigma(O)
    &=\frac{1}{1+e^{2}}=0.119\\
    \frac{\partial L}{\partial w_x}
    &=-2*(1-0.119)*0.119*(1-0.119)*1=-0.184\\
    \frac{\partial L}{\partial w_y}
    &=-2*(1-0.119)*0.119*(1-0.119)*-1=0.184\\
    t&=1\\
    \intertext{Calculating for $w_x$}
    s&=\rho1*s+(1-\rho1)*g=0.9*0+(1-0.9)*(-0.184)=-0.0184\\
    r&=\rho2*r+(1-\rho2)g*g=0.99*0+(1-0.99)*(-0.184)(-0.184)=0.000338\\
    \hat{s}&=\frac{s}{1-\rho1^{t}}=-0.0184/1-0.9^{1}=-0.184\\
    \hat{r}&=\frac{r}{1-\rho2^{t}}=0.000338/1-0.99^{1}=0.0338\\
    \Delta\theta_x&=-\epsilon*\frac{\hat{s}}{\sqrt{\hat{r}}+\delta}=-1*\frac{-0.184}{\sqrt{0.0338}+10^{-8}}=0.184/0.183=1.005
    \intertext{Calculating for $w_y$}
    s&=\rho1*s+(1-\rho1)*g=0.9*0+(1-0.9)*(0.184)=0.0184\\
    r&=\rho2*r+(1-\rho2)g*g=0.99*0+(1-0.99)*(0.184)(0.184)=0.000338\\
    \hat{s}&=\frac{s}{1-\rho1^{t}}=0.0184/1-0.9^{1}=0.184\\
    \hat{r}&=\frac{r}{1-\rho2^{t}}=0.000338/1-0.99^{1}=0.0338\\
    \Delta\theta_y&=\epsilon*\frac{\hat{s}}{\sqrt{\hat{r}}+\delta}=-1*\frac{0.184}{\sqrt{0.0338}+10^{-8}}=-0.184/0.183=-1.005\\
    w_x&=-1+1.005=0.005\\
    w_y&=1-1.005=-0.005
   \intertext{\textbf{For 2nd iteration}}
    O(x,y)
    &=w_x*x+w_y*y=0.005*1-0.005*-1=0.01\\
    \sigma(O)
    &=\frac{1}{1+e^{-0.01}}=0.502\\
    \frac{\partial L}{\partial w_x}
    &=-2*(1-0.502)*0.502*(1-0.502)*1=-0.248\\
    \frac{\partial L}{\partial w_y}
    &=-2*(1-0.502)*0.502*(1-0.502)*-1=0.248\\
    t&=2\\
    \intertext{Calculating for $w_x$}
    s&=\rho1*s+(1-\rho1)*g=0.9*(-0.0184)+(1-0.9)*(-0.248)=-0.0413\\ 
    r&=\rho2*r+(1-\rho2)g*g=0.99*0.000338+(1-0.99)*(-0.248)(-0.248)=0.000949\\
    \hat{s}&=\frac{s}{1-\rho1^{t}}=-0.0413/1-0.9^{2}=-0.217\\ 
    \hat{r}&=\frac{r}{1-\rho2^{t}}=0.000949/1-0.99^{2}=0.0476\\
    \Delta\theta_x&=-\epsilon*\frac{\hat{s}}{\sqrt{\hat{r}}+\delta}=-1*\frac{-0.217}{\sqrt{0.0476}+10^{-8}}=0.217/0.218=0.995
    \intertext{Calculating for $w_y$}
    s&=\rho1*s+(1-\rho1)*g=0.9*0.0184+(1-0.9)*(0.248)=0.0413\\
    r&=\rho2*r+(1-\rho2)g*g=0.99*0.000338+(1-0.99)*(0.248)(0.248)=0.000949\\
    \hat{s}&=\frac{s}{1-\rho1^{t}}=0.0413/1-0.9^{2}=0.217\\
    \hat{r}&=\frac{r}{1-\rho2^{t}}=0.000949/1-0.99^{2}=0.0476\\
    \Delta\theta_y&=-\epsilon*\frac{\hat{s}}{\sqrt{\hat{r}}+\delta}=-1*\frac{0.217}{\sqrt{0.0476}+10^{-8}}=-0.217/0.218=-0.995\\
    w_x&=0.005+0.995=1\\
    w_y&=-0.005-0.995=-1
    \intertext{\textbf{For 3rd iteration :}}
    O(x,y)
    &=w_x*x+w_y*y=1*1-1*-1=2\\ 
    \sigma(O)
    &=\frac{1}{1+e^{-2}}=0.881\\ 
    \frac{\partial L}{\partial w_x}
    &=-2*(1-0.881)*0.881*(1-0.881)*1=-0.02\\ 
    \frac{\partial L}{\partial w_y}
    &=-2*(1-0.881)*0.881*(1-0.881)*-1=0.02\\
    t&=3\\
    \intertext{Calculating for $w_x$}
    s&=\rho1*s+(1-\rho1)*g=0.9*(-0.0413)+(1-0.9)*(-0.02)=-0.039\\  
    r&=\rho2*r+(1-\rho2)g*g=0.99*0.000949+(1-0.99)*(-0.02)(-0.02)=0.000943\\
    \hat{s}&=\frac{s}{1-\rho1^{t}}=-0.039/1-0.9^{3}=-0.143\\ 
    \hat{r}&=\frac{r}{1-\rho2^{t}}=0.000943/1-0.99^{3}=0.0316\\ 
    \Delta\theta_x&=-\epsilon*\frac{\hat{s}}{\sqrt{\hat{r}}+\delta}=-1*\frac{-0.143}{\sqrt{0.0316}+10^{-8}}=0.143/0.177=0.807
    \intertext{Calculating for $w_y$}
    s&=\rho1*s+(1-\rho1)*g=0.9*0.0413+(1-0.9)*(0.02)=0.039\\
    r&=\rho2*r+(1-\rho2)g*g=0.99*0.000949+(1-0.99)*(0.02)(0.02)=0.000943\\
    \hat{s}&=\frac{s}{1-\rho1^{t}}=0.039/1-0.9^{3}=0.143\\
    \hat{r}&=\frac{r}{1-\rho2^{t}}=0.000943/1-0.99^{3}=0.0316\\
    \Delta\theta_y&=-\epsilon*\frac{\hat{s}}{\sqrt{\hat{r}}+\delta}=-1*\frac{0.143}{\sqrt{0.0316}+10^{-8}}=-0.143/0.177=-0.807\\
    w_x&=1+0.807=1.807\\
    w_y&=-1-0.807=-1.807
\end{align*}

\section{Unstable Gradient Problem}
1.
        $\frac{dh_n}{dw_i} = \frac{dh_n}{dh_{n-1}} * \frac{dh_{n-1}}{dh_{n-2}} \ldots  \frac{dh_{i+1}}{dh_{i}} * \frac{dh_i}{dw_i}$\\\\
2. for sigmoid derivative defined as: 
        \begin{align*}
            \frac{dh_n}{dw_i} = [\Pi_{k = i+1}^{n}  h_k (1 - h_k) w_k ] h_i (1 - h_i) h_{i-1}  
        \end{align*}
        The gradient will decay quickly. Because maximum derivative $<$ 1 \\\\
    for relu derivative defined as when less than zero then gradients will vanish and when greater than zero: $\frac{dh_n}{dw_i} = [\Pi_{k = i+1}^{n} w_k] h_{i-1}$\\. That is why leakyReLU is used to avoid vanished gradients when less than 0.\\
\\
3. $Var(\hat{X}.\hat{Y}) = E(\hat{X}^2.\hat{Y}^2) - [E(\hat{X}.\hat{Y})]^2 = E(\hat{X})^2Var(\hat{Y}) + E(\hat{Y})^2Var(\hat{X}) + Var(\hat{X})Var(\hat{Y}) = Var(\hat{X})Var(\hat{Y})$\\
as $E(\hat{X}) = 0$ and $E(\hat{Y}) = 0$\\
\\
So, $Var(\hat{X_1}.\hat{X_2}...\hat{X_n}) = \prod_i Var(\hat{X_i})$\\
\\
4. $h^{i}_{j} = \sum_k W^{i}_{j,k}h^{i-1}$\\\\
$Var(h^{i}_{j}) = Var(\sum_k W^{i}_{j,k})Var(h^{i-1})$\\\\
$Var(h^{i}_{j}) = n_i Var(W^{i})Var(h^{i-1})$\\\\
since the variance is same for all weights.\\
\\
5.$Var(h^{i}_{j}) = n_i Var(W^{i})Var(h^{i-1})$\\\\
$1 = n_i Var(W^{i})$ as $Var(h^{i}_{j}) = Var(h^{i-1})$\\\\
$Var(W^{i}) = \frac{1}{n_i} $\\\\
6. $\delta^{i} = W^{i+1}\delta^{i+1}$\\\\
$\frac{dh_n}{dh_i} = W^{i+1}\frac{dh_n}{dh_{i+1}}$\\\\
$Var(\frac{dh_n}{dh_i}) = Var(W^{i+1})Var(\frac{dh_n}{dh_{i+1}})$\\\\
$Var(W^{i}) = \frac{1}{n_i} $\\\\

\end{document}
